pcuic/theories/PCUICValidity.v
@@ -1,17 +1,30 @@
-From Coq Require Import String Bool List PeanoNat Lia.
+From Coq Require Import String Bool List PeanoNat Lia Morphisms.
 From MetaCoq.Template Require Import config utils.
 From MetaCoq.PCUIC Require Import PCUICAst
      PCUICLiftSubst PCUICTyping PCUICWeakeningEnv PCUICWeakening PCUICInversion
      PCUICSubstitution PCUICReduction PCUICCumulativity PCUICGeneration PCUICUnivSubst
      PCUICParallelReductionConfluence
      PCUICUnivSubstitution PCUICConversion PCUICContexts PCUICArities
-     PCUICSpine PCUICInductives.
+     PCUICSpine PCUICInductives PCUICContexts
+     PCUICSigmaCalculus PCUICClosed.
 
 From Equations Require Import Equations.
 Require Import Equations.Prop.DepElim.
 Require Import ssreflect.
 
 Derive Signature for typing cumul.
+
+Instance proper_inst' : Proper (`=1` ==> pointwise_relation _ Logic.eq) inst.
+Proof.
+  intros f f' Hff' t. now apply inst_ext.
+Qed.
+
+Instance Proper_map_ho {A B} : Proper ((pointwise_relation A Logic.eq) ==> Logic.eq ==> Logic.eq)
+  (@map A B).
+Proof.
+  intros f g Hfg x y ->. apply map_ext.
+  apply Hfg.
+Qed.
 
 Section Validity.
   Context `{cf : config.checker_flags}.
@@ -288,38 +301,64 @@ Section Validity.
       rewrite subst_context_app. simpl.  unfold app_context. f_equal.
   Qed.
 
-  Lemma wf_local_smash_context_gen Σ Γ Δ :
+  Lemma wf_local_rel_smash_context_gen Σ Γ Δ Δ' :
     wf Σ.1 ->
-    wf_local Σ Γ -> All_local_env (fun Δ => lift_typing typing Σ (Γ ,,, Δ)) Δ -> 
-    wf_local Σ (smash_context Δ Γ).
+    wf_local Σ (Δ' ,,, Γ) -> 
+    wf_local_rel Σ (Δ' ,,, Γ) Δ ->
+    wf_local_rel Σ Δ' (smash_context Δ Γ).
   Proof.
     intros wfΣ.
-    induction 1 in Δ |- *; simpl; auto.
-    - intros wfΔ. eapply (All_local_env_impl _ _ _ wfΔ).
-      intros. now rewrite app_context_nil_l in X.
-    - intros a.
-      apply IHX. eapply All_local_env_app_inv. split; auto.
+    induction Γ in Δ |- *; simpl; auto.
+    intros wfΓ wfΔ. depelim wfΓ; simpl.
+    - apply IHΓ; auto. eapply All_local_env_app_inv. split; auto.
       repeat constructor; auto.
       eapply All_local_env_impl; eauto. simpl; intros.
+      unfold lift_typing in X |- *.
       now rewrite app_context_assoc.
-    - intros a.
-      apply IHX. eapply All_local_env_subst; eauto. simpl; intros.
-      destruct T; unfold lift_typing in *; simpl in *; firstorder auto.
+    - apply IHΓ. auto. eapply All_local_env_subst; eauto. simpl; intros.
+      destruct T; unfold lift_typing in X |- *; simpl in *; firstorder auto.
       rewrite Nat.add_0_r.
-      eapply (substitution _ Γ [vdef na b t] [b] Γ0) in X0; eauto.
+      eapply (substitution _ (Δ' ,,, Γ) [vdef na b t] [b] Γ0) in X; eauto.
       rewrite -{1}(subst_empty 0 b). repeat constructor. now rewrite !subst_empty.
       exists x.
       rewrite Nat.add_0_r.
-      eapply (substitution _ Γ [vdef na b t] [b] Γ0) in p; eauto.
+      eapply (substitution _ _ [vdef na b t] [b] Γ0) in p; eauto.
       rewrite -{1}(subst_empty 0 b). repeat constructor. now rewrite !subst_empty.
   Qed.
+
+  Lemma wf_local_rel_smash_context Σ Γ Δ :
+    wf Σ.1 ->
+    wf_local Σ (Δ ,,, Γ) -> 
+    wf_local_rel Σ Δ (smash_context [] Γ).
+  Proof.
+    intros. eapply wf_local_rel_smash_context_gen; eauto. constructor.
+  Qed.
   
+  Lemma wf_local_rel_empty Σ Γ : wf_local_rel Σ [] Γ <~> wf_local Σ Γ.
+  Proof.
+    split.
+    - intros h. eapply (All_local_env_impl _ _ _ h). firstorder.
+      red in X |- *. now rewrite app_context_nil_l in X.
+    - intros h. eapply (All_local_env_impl _ _ _ h). firstorder.
+      red in X |- *. now rewrite app_context_nil_l.
+  Qed.
+
   Lemma wf_local_smash_context Σ Γ :
     wf Σ.1 -> wf_local Σ Γ -> wf_local Σ (smash_context [] Γ).
   Proof.
-    intros; eapply wf_local_smash_context_gen; eauto.
+    intros; apply wf_local_rel_empty. eapply (wf_local_rel_smash_context Σ Γ []); 
+      rewrite ?app_context_nil_l; eauto.
   Qed.
 
+  Lemma context_assumptions_smash_context Δ Γ :
+    context_assumptions (smash_context Δ Γ) = 
+    context_assumptions Δ + context_assumptions Γ.
+  Proof.
+    induction Γ as [|[? [] ?] ?] in Δ |- *; simpl; auto;
+    rewrite IHΓ.
+    - now rewrite context_assumptions_fold.
+    - rewrite context_assumptions_app /=. lia.
+  Qed. 
 
   Lemma nth_error_ass_subst_context s k Γ : 
     (forall n d, nth_error Γ n = Some d -> decl_body d = None) ->
@@ -381,7 +420,6 @@ Section Validity.
   *)
 
   Local Open Scope sigma.
-  Require Import PCUICSigmaCalculus PCUICClosed.
   Lemma Upn_compose n σ σ' : ⇑^n σ ∘s ⇑^n σ' =1 ⇑^n (σ ∘s σ').
   Proof.
     induction n. unfold Upn. simpl.
@@ -389,48 +427,6 @@ Section Validity.
     rewrite !Upn_S. autorewrite with sigma. now rewrite IHn.
   Qed.
 
-  Fixpoint extended_subst (Γ : context) (n : nat) :=
-    match Γ with
-    | nil => nil
-    | cons d vs =>
-      match decl_body d with
-      | Some b =>
-        (* Δ , vs |- b *)
-        let s := extended_subst vs n in
-        (* Δ , smash_context vs |- s : vs *)
-        let b' := subst0 s (lift (context_assumptions vs) #|s| b) in
-        (* Δ, smash_context vs |- b' *)
-        b' :: s
-      | None => tRel n :: extended_subst vs (S n)
-      end
-    end.
-
-  Lemma extended_subst_length Γ n : #|extended_subst Γ n| = #|Γ|.
-  Proof.
-    induction Γ in n |- *; simpl; auto.
-    now destruct a as [? [?|] ?] => /=; simpl; rewrite IHΓ. 
-  Qed.
-  Hint Rewrite extended_subst_length : len.
-  (* Lemma Up_compose σ s : ⇑ σ ∘s (s ⋅n ids) *)
-
-  Lemma extended_subst_lift (Δ : context) n : 
-    extended_subst Δ n = map (lift0 n) (extended_subst Δ 0).
-  Proof.
-    rewrite -{1}(Nat.add_0_r n).
-    generalize 0 at 1 3. revert n.
-    induction Δ.
-    simpl. auto.
-    intros n n'.
-    destruct a as [na [?|] ?]. simpl.
-    f_equal. 2:auto.
-    specialize (IHΔ n n').
-    rewrite IHΔ.
-    rewrite (distr_lift_subst _ _ n 0).
-    rewrite extended_subst_length Nat.add_0_r.
-    admit.
-    simpl. f_equal; auto. specialize (IHΔ n (S n')).
-    now rewrite -Nat.add_succ_r.
-  Admitted.
 
   Hint Rewrite Nat.add_0_r : len.
 
@@ -501,11 +497,58 @@ Section Validity.
     apply nth_error_None in Heq'. lia.
   Qed.
 
-  Lemma inst_extended_subst_shift_ind (Γ : context) k : 
-    closed_ctx Γ ->
-    (forall x, x < #|Γ| -> 
-      option_map (fun x0 : term => x0.[↑^k]) (nth_error (extended_subst Γ 0) x) =
-      nth_error (extended_subst Γ k) x) ->
+  Fixpoint extended_subst (Γ : context) (n : nat) 
+   (* Δ, smash_context Γ, n |- extended_subst Γ n : Γ *) :=
+    match Γ with
+    | nil => nil
+    | cons d vs =>
+      match decl_body d with
+      | Some b =>
+        (* Δ , vs |- b *)
+        let s := extended_subst vs n in
+        (* Δ , smash_context vs , n |- s : vs *)
+        let b' := lift (context_assumptions vs + n) #|s| b in
+        (* Δ, smash_context vs, n , vs |- b' *)
+        let b' := subst0 s b' in
+        (* Δ, smash_context vs , n |- b' *)
+        b' :: s
+      | None => tRel n :: extended_subst vs (S n)
+      end
+    end.
+
+  Lemma extended_subst_length Γ n : #|extended_subst Γ n| = #|Γ|.
+  Proof.
+    induction Γ in n |- *; simpl; auto.
+    now destruct a as [? [?|] ?] => /=; simpl; rewrite IHΓ. 
+  Qed.
+  Hint Rewrite extended_subst_length : len.
+
+
+
+  Hint Rewrite idsn_length : len.
+
+  Lemma subst_fn_eq s s' x : s = s' -> subst_fn s x = subst_fn s' x.
+  Proof.
+    intros -> ; reflexivity.
+  Qed.
+
+  Lemma lift_extended_subst (Γ : context) k : 
+    extended_subst Γ k = map (lift0 k) (extended_subst Γ 0).
+  Proof.
+    induction Γ as [|[? [] ?] ?] in k |- *; simpl; auto.
+    - rewrite IHΓ. f_equal.
+      autorewrite with len.
+      rewrite distr_lift_subst. f_equal.
+      autorewrite with len. rewrite simpl_lift. lia. lia.
+      f_equal; lia.
+    - rewrite Nat.add_0_r; f_equal.
+      rewrite IHΓ (IHΓ 1).
+      rewrite map_map_compose. apply map_ext => x.
+      rewrite simpl_lift; try lia.
+      now rewrite Nat.add_1_r.
+  Qed.
+  
+  Lemma inst_extended_subst_shift (Γ : context) k : 
     map (inst ((extended_subst Γ 0 ⋅n ids) ∘s ↑^k)) (idsn #|Γ|) =
     map (inst (extended_subst Γ k ⋅n ids)) (idsn #|Γ|).
   Proof.
@@ -521,80 +564,22 @@ Section Validity.
     unfold subst_compose. rewrite Hσ'.
     apply some_inj.
     rewrite -Hd. change (Some d'.[↑^k]) with (option_map (fun x => inst (↑^k) x) (Some d')).
-    rewrite -Hd'. now apply H0.
-  Qed.
-
-  Hint Rewrite idsn_length : len.
-
-  Lemma subst_fn_eq s s' x : s = s' -> subst_fn s x = subst_fn s' x.
-  Proof.
-    intros -> ; reflexivity.
-  Qed.
-
-  Lemma extended_subst_shift (Γ : context) k : 
-    closed_ctx Γ ->
-    forall x, x < #|Γ| -> 
-    option_map (fun x0 : term => x0.[↑^k]) (nth_error (extended_subst Γ 0) x) =
-    nth_error (extended_subst Γ k) x.
-  Proof.
-    intros clΓ.
-    induction Γ in k, clΓ |- *. simpl. lia.
-    simpl; intros x Hx.
-    intros. 
-    destruct a as [? [] ?]; auto.
-    simpl.
-    autorewrite with sigma.
-    rewrite !ren_lift_renaming. autorewrite with len.
-    rewrite Upn_eq. rewrite !subst_consn_compose.
-    autorewrite with sigma.
-    move/closedn_ctx_cons/andP: clΓ => [clΓ /andP [clt _]].
-    simpl in clt.
-    destruct x. simpl. f_equal.
-    autorewrite with sigma.
-    rewrite subst_consn_compose.
-    eapply inst_ext_closed; eauto.
-    intros.
-    apply subst_consn_eq; autorewrite with len; auto.
-    pose proof (inst_extended_subst_shift_ind Γ k clΓ).
-    rewrite -H0. intros. apply IHΓ; auto.
-    rewrite map_map_compose. apply subst_fn_eq.
-    apply map_ext. intros.
+    rewrite -Hd'.
+    rewrite (lift_extended_subst _ k).
+    rewrite nth_error_map. apply option_map_ext => t.
     now autorewrite with sigma.
-
-    simpl. apply IHΓ; auto. lia.
-
-    simpl.
-    destruct x; simpl. unfold shiftk.
-    now rewrite Nat.add_0_r.
-    move/closedn_ctx_cons/andP: clΓ => [clΓ /andP [clt _]].
-    rewrite -(IHΓ (S k)); auto. lia.
-    rewrite -(IHΓ 1 clΓ x ltac:(lia)).
-    rewrite option_map_two. apply option_map_ext.
-    intros. autorewrite with sigma.
-    now rewrite -shiftk_shift -shiftk_shift_l.
-  Qed.
-
-  Lemma inst_extended_subst_shift (Γ : context) k : 
-    closed_ctx Γ ->
-    map (inst ((extended_subst Γ 0 ⋅n ids) ∘s ↑^k)) (idsn #|Γ|) =
-    map (inst (extended_subst Γ k ⋅n ids)) (idsn #|Γ|).
-  Proof.
-    intros. apply inst_extended_subst_shift_ind; auto.
-    now apply extended_subst_shift.
   Qed.
 
   Lemma smash_context_acc Γ Δ : 
-    closed_ctx Γ ->
     smash_context Δ Γ =
         subst_context (extended_subst Γ 0) 0 (lift_context (context_assumptions Γ) #|Γ| Δ)
      ++ smash_context [] Γ.
   Proof.
     revert Δ.
-    induction Γ as [|[? [] ?] ?]; intros Δ cl.
+    induction Γ as [|[? [] ?] ?]; intros Δ.
     - simpl; auto.
       now rewrite subst0_context app_nil_r lift0_context.
     - simpl. autorewrite with len.
-      move/closedn_ctx_cons/andP: cl => [clΓ /andP [clt _]].
       rewrite IHΓ; auto.
       rewrite subst_context_nil. f_equal.
       rewrite (subst_context_decompo [_] _).
@@ -618,7 +603,6 @@ Section Validity.
       reflexivity.
       
     - simpl.
-      move/closedn_ctx_cons/andP: cl => [clΓ /andP [clt _]].
       rewrite IHΓ /=. auto.
       rewrite (IHΓ [_]). auto. rewrite !app_assoc. f_equal.
       rewrite app_nil_r. unfold map_decl. simpl. unfold app_context.
@@ -642,7 +626,7 @@ Section Validity.
       autorewrite with sigma.
       apply subst_cons_proper. auto.
       rewrite !Upn_eq. autorewrite with sigma.
-      rewrite !subst_consn_compose.
+      rewrite subst_consn_compose.
       setoid_rewrite subst_consn_compose at 2 3.
       apply subst_consn_proper.
       rewrite -inst_extended_subst_shift; auto.
@@ -671,73 +655,400 @@ Section Validity.
   Lemma skipn_0_eq {A} (l : list A) n : n =  0 -> skipn n l = l.
   Proof. intros ->; apply PCUICAstUtils.skipn_0. Qed.
  
+  Lemma map_subst_app_decomp (l l' : list term) (k : nat) (ts : list term) :
+    map (subst (l ++ l') k) ts = map (fun x => subst l' k (subst (map (lift0 #|l'|) l) k x)) ts.
+  Proof.
+    apply map_ext. apply subst_app_decomp.
+  Qed.
+ 
+  Lemma map_reln_ext (f g : term -> term) k Γ :
+    (forall n, n < #|Γ| -> f (tRel (k + n)) = g (tRel (k + n))) ->
+    map f (reln [] k Γ) = map g (reln [] k Γ).
+  Proof.
+    intros Hf.
+    induction Γ as [|[? [] ?] ?] in k, Hf |- *; simpl; auto.
+    - rewrite reln_acc map_app. simpl.
+      rewrite map_app /=. rewrite IHΓ //.
+      intros. simpl in Hf. specialize (Hf (S n)).
+      forward Hf. lia. rewrite -Nat.add_assoc. apply Hf.
+    - rewrite reln_acc map_app. simpl.
+      rewrite map_app /= IHΓ //.
+      intros. simpl in Hf. specialize (Hf (S n)).
+      forward Hf. lia. rewrite -Nat.add_assoc. apply Hf.
+      f_equal. f_equal. specialize (Hf 0). simpl in Hf.
+      forward Hf by lia. now rewrite Nat.add_0_r in Hf.
+  Qed.
+
   Lemma extended_subst_to_extended_list_k Γ k :
-    (map (subst0 (extended_subst Γ k)) (to_extended_list_k Γ k)) = 
+    (map (subst (extended_subst Γ 0) k) (to_extended_list_k Γ k)) = 
     to_extended_list_k (smash_context [] Γ) k.
   Proof.
+    unfold to_extended_list_k.
     induction Γ in k |- *. simpl. reflexivity.
-    unfold to_extended_list_k. simpl.
-    destruct a as [? [] ?]; simpl. admit.
-  Admitted.
+    destruct a as [? [] ?]; simpl.
+    - rewrite smash_context_acc //.
+      rewrite reln_app. autorewrite with len. simpl.
+      rewrite -IHΓ //. rewrite Nat.add_1_r.
+      rewrite (reln_lift 1). 
+      clear.
+      rewrite (map_subst_app_decomp [_]).
+      rewrite -map_map_compose. f_equal.
+      simpl.
+      generalize (lift0 #|extended_subst Γ 0| 
+        (subst0 (extended_subst Γ 0) (lift (context_assumptions Γ) #|Γ| t))).
+      intros t0.
+      change 1 with #|[t0]|.
+      generalize [t0]. clear.
+      intros l. generalize (Nat.le_refl k).
+      generalize k at 1 3.
+      induction Γ as [|[? [] ?] ?] in k, l |- *; simpl. reflexivity.
+      simpl. intros k0 lek0. apply IHΓ. lia.
+      intros k0 lek0. rewrite reln_acc map_app. simpl.
+      rewrite map_app. simpl.
+      elim: leb_spec_Set => Hle. f_equal. apply IHΓ. lia.
+      f_equal. elim: nth_error_spec => [x Hx Hl|Hl]. lia.
+      f_equal. lia. lia.
+    - rewrite smash_context_acc //.
+      simpl.
+      rewrite reln_acc map_app.
+      rewrite (reln_acc [_] _ (smash_context [] Γ)). 
+      simpl. rewrite Nat.leb_refl Nat.sub_diag /=. f_equal.
+      rewrite -IHΓ //.
+      2:{ do 2 f_equal; lia. }
+      apply map_reln_ext => n Hn.
+      rewrite lift_extended_subst //.
+      replace (k + 1 + n) with (S (k + n)) by lia.
+      simpl.
+      elim: leb_spec_Set => Hle; [|lia].
+      elim: leb_spec_Set => Hle'; [|lia].
+      replace (S (k + n) - k) with (S n) by lia.
+      replace (S (k + n) - (k + 1)) with n by lia.
+      simpl.
+      rewrite nth_error_map.
+      elim: nth_error_spec => [x Hx Hlen|Hlen].
+      simpl. rewrite simpl_lift; try lia. f_equal. simpl.
+      autorewrite with len in Hlen. lia.
+  Qed.
 
+  Hint Rewrite smash_context_length arities_context_length : len.
+
+  Lemma assumption_context_fold f Γ :
+    assumption_context Γ -> assumption_context (fold_context f Γ).
+  Proof. 
+    induction 1; simpl. constructor. rewrite fold_context_snoc0.
+    now constructor.
+  Qed.
+  
+  Lemma option_map_Some {A B} (f : A -> B) (o : option A) x : 
+    option_map f o = Some x ->
+    ∑ y, (o = Some y) * (x = f y).
+  Proof.
+    destruct o => /= //.
+    move=> [] <-. exists a; auto.
+  Qed.
+
+  Lemma map_subst_closedn (s : list term) (k : nat) l :
+    forallb (closedn k) l -> map (subst s k) l = l.
+  Proof.
+    induction l; simpl; auto.
+    move/andP=> [cla cll]. rewrite IHl //.
+    now rewrite subst_closedn.
+  Qed.
+
+  Lemma closedn_extended_subst_gen Γ k k' : 
+    closedn_ctx k Γ -> 
+    forallb (closedn (k' + k + context_assumptions Γ)) (extended_subst Γ k').
+  Proof.
+    induction Γ as [|[? [] ?] ?] in k, k' |- *; simpl; auto;
+    rewrite ?closedn_ctx_cons;
+     move/andP => [clΓ /andP[clb clt]].
+    - rewrite IHΓ //.
+      epose proof (closedn_subst (extended_subst Γ k') (k' + k + context_assumptions Γ) 0).
+      autorewrite with len in H. rewrite andb_true_r.
+      eapply H; auto.
+      replace (k' + k + context_assumptions Γ + #|Γ|)
+      with (k + #|Γ| + (context_assumptions Γ + k')) by lia.
+      eapply closedn_lift. eapply clb.
+    - apply andb_and. split.
+      * apply Nat.ltb_lt; lia.
+      * specialize (IHΓ k (S k') clΓ).
+        red. rewrite -IHΓ. f_equal. f_equal. lia.
+  Qed.
+
+  Lemma closedn_extended_subst Γ : 
+    closed_ctx Γ -> 
+    forallb (closedn (context_assumptions Γ)) (extended_subst Γ 0).
+  Proof.
+    intros clΓ. now apply (closedn_extended_subst_gen Γ 0 0).
+  Qed.
+
+  Lemma closedn_ctx_lift n k k' Γ : closedn_ctx k Γ ->
+    closedn_ctx (n + k) (lift_context n k' Γ).
+  Proof.
+    induction Γ as [|d ?]; simpl; auto; rewrite lift_context_snoc !closedn_ctx_cons /=;
+      move/andP=> [clΓ cld]; rewrite IHΓ //;
+    autorewrite with len in cld.
+    move: cld;  rewrite /closed_decl. simpl.
+    move/andP=> [clb clt]; apply andb_and; split.
+    destruct (decl_body d) => /= //. simpl in clb |- *.
+    eapply (closedn_lift n) in clb.
+    autorewrite with len. now rewrite -Nat.add_assoc Nat.add_comm.
+    eapply (closedn_lift n) in clt.
+    autorewrite with len. now rewrite -Nat.add_assoc Nat.add_comm.
+  Qed.
+
+  Lemma closedn_ctx_subst k k' s Γ : 
+    closedn_ctx (k + k' + #|s|) Γ ->
+    forallb (closedn k) s ->
+    closedn_ctx (k + k') (subst_context s k' Γ).
+  Proof.
+    induction Γ as [|d ?] in k' |- *; simpl; auto; rewrite subst_context_snoc !closedn_ctx_cons /=;
+    move/andP=> [clΓ cld]  cls; rewrite IHΓ //;
+    autorewrite with len in cld.
+    move: cld;  rewrite /closed_decl. simpl.
+    move/andP=> [clb clt]; apply andb_and; split.
+    destruct (decl_body d) => /= //. simpl in clb |- *.
+    rewrite -Nat.add_assoc [#|s| + _]Nat.add_comm Nat.add_assoc in clb.
+    rewrite -(Nat.add_assoc k) in clb.
+    eapply (closedn_subst s) in clb => //. rewrite Nat.add_assoc in clb.
+    autorewrite with len. now rewrite (Nat.add_comm #|Γ|).
+    rewrite -Nat.add_assoc [#|s| + _]Nat.add_comm Nat.add_assoc in clt.
+    rewrite -(Nat.add_assoc k) in clt.
+    eapply (closedn_subst s) in clt => //. rewrite Nat.add_assoc in clt.
+    autorewrite with len. now rewrite (Nat.add_comm #|Γ|).
+  Qed.
+
+  Lemma assumption_context_skipn Γ n : 
+    assumption_context Γ -> 
+    assumption_context (skipn n Γ).
+  Proof.
+    induction 1 in n |- *; simpl.
+    - destruct n; constructor.
+    - destruct n. rewrite skipn_0. constructor; auto.
+      now rewrite skipn_S.
+  Qed. 
+
+  Lemma skipn_eq_cons {A} n (l : list A) hd tl : skipn n l = hd :: tl ->
+    (nth_error l n = Some hd) * (skipn (S n) l = tl).
+  Proof.
+    induction n in l, hd, tl |- *.
+    - rewrite skipn_0 => ->. simpl. now rewrite skipn_S skipn_0.
+    - destruct l as [|hd' tl'].
+      * rewrite skipn_nil. discriminate.
+      * rewrite skipn_S. rewrite skipn_S. simpl.
+        apply IHn.
+  Qed.
+
+  (* k is the projection number: 0 is the first argument *)
+  Definition projection_type mdecl ind k ty := 
+    let u := PCUICLookup.abstract_instance (PCUICEnvironment.ind_universes mdecl) in
+    let indsubst := inds (inductive_mind ind) u (ind_bodies mdecl) in
+    let projsubst := projs ind (ind_npars mdecl) k in
+    subst indsubst (S (ind_npars mdecl))
+        (subst0 projsubst (lift 1 k 
+          (subst (extended_subst (ind_params mdecl) 0) k
+           (lift (context_assumptions (ind_params mdecl)) (k + #|ind_params mdecl|)
+            ty)))).
+            
+  Definition projection_type' mdecl ind k ty :=
+    let u := PCUICLookup.abstract_instance (PCUICEnvironment.ind_universes mdecl) in
+    let indsubst := inds (inductive_mind ind) u (ind_bodies mdecl) in
+    let projsubst := projs ind (ind_npars mdecl) k in
+    (subst0 projsubst
+      (subst (extended_subst (ind_params mdecl) 0) (S k)
+      (lift 1 k (subst indsubst (k + #|ind_params mdecl|) ty)))).
+ 
+  Definition projection_decl_type mdecl ind k ty := 
+    let u := PCUICLookup.abstract_instance (PCUICEnvironment.ind_universes mdecl) in
+    let indsubst := inds (inductive_mind ind) u (ind_bodies mdecl) in
+    let projsubst := projs ind (ind_npars mdecl) k in
+    subst indsubst (S (ind_npars mdecl))
+        (subst0 projsubst (lift 1 k ty)).
+
+  Lemma nth_error_Some' {A} l n : (∑ x : A, nth_error l n = Some x) <~> n < length l.
+  Proof.
+    revert n. induction l; destruct n; simpl.
+    - split; [now destruct 1 | intros H'; elimtype False; inversion H'].
+    - split; [now destruct 1 | intros H'; elimtype False; inversion H'].
+    - split; now intuition eauto with arith.
+    - destruct (IHl n); split; auto with arith.
+  Qed.
+
+  Lemma on_projections_decl {Σ mdecl ind idecl cs} :
+    forall (Hdecl : declared_inductive Σ mdecl ind idecl) (wfΣ : wf Σ),
+    let oib := declared_inductive_inv weaken_env_prop_typing wfΣ wfΣ Hdecl in
+    let u := PCUICLookup.abstract_instance (ind_universes mdecl) in
+    on_projections mdecl (inductive_mind ind) (inductive_ind ind) idecl (oib.(ind_indices)) cs ->
+    Alli (fun i decl => 
+      ∑ pdecl, 
+        (nth_error (ind_projs idecl) (context_assumptions (cshape_args cs) - S i) = Some pdecl))
+      0 (smash_context [] cs.(cshape_args)).
+  Proof.
+    intros.
+    destruct X as [_ _ _ on_projs_all on_projs].
+    eapply forall_nth_error_Alli.
+    intros.
+    pose proof (equiv_inv _ _ (nth_error_Some' (ind_projs idecl) (context_assumptions (cshape_args cs) - S i))).
+    apply X. eapply nth_error_Some_length in H. 
+      autorewrite with len in H. simpl in H; lia.
+  Qed.
+
+  Lemma consistent_instance_ext_abstract_instance Σ mdecl mind :
+    wf Σ ->
+    declared_minductive Σ mind mdecl ->
+    consistent_instance_ext (Σ, ind_universes mdecl) (ind_universes mdecl)
+       (PCUICLookup.abstract_instance (ind_universes mdecl)).
+  Proof.
+    todo "universes"%string.
+  Defined.
+
+  Lemma to_extended_list_length Γ : #|to_extended_list Γ| = context_assumptions Γ.
+  Proof. now rewrite /to_extended_list PCUICCtxShape.to_extended_list_k_length. Qed.
+  Hint Rewrite to_extended_list_length List.rev_length : len.
+
+  Lemma subst_id s Γ t : 
+    closedn #|s| t ->
+    assumption_context Γ ->
+    s = List.rev (to_extended_list Γ) ->
+    subst s 0 t = t.
+  Proof.
+    intros cl ass eq.
+    autorewrite with sigma.
+    rewrite -{2}(subst_ids t).
+    eapply inst_ext_closed; eauto.
+    intros.
+    unfold ids, subst_consn. simpl.
+    destruct (equiv_inv _ _ (nth_error_Some' s x) H). rewrite e.
+    subst s.
+    rewrite /to_extended_list /to_extended_list_k in e.
+    rewrite List.rev_length in cl, H. autorewrite with len in *.
+    rewrite reln_alt_eq in e.
+    rewrite app_nil_r List.rev_involutive in e.
+    clear -ass e. revert e.
+    rewrite -{2}(Nat.add_0_r x).
+    generalize 0.
+    induction Γ in x, ass, x0 |- * => n. simpl in *. rewrite nth_error_nil => //.
+    depelim ass; simpl.
+    destruct x. simpl in *. congruence.
+    move=> e; specialize (IHΓ ass); simpl in e.
+    specialize (IHΓ _ _ _ e). subst x0. f_equal. lia.
+  Qed.
+  
+  Lemma isType_closed {Σ Γ T} : wf Σ.1 -> isType Σ Γ T -> closedn #|Γ| T.
+  Proof. intros wfΣ [s Hs]. now eapply subject_closed in Hs. Qed.
+
+  Lemma subst_instance_context_id Σ univs Γ : 
+    let u :=  PCUICLookup.abstract_instance univs in
+    wf_local (Σ, univs) Γ ->
+    subst_instance_context u Γ = Γ.
+  Proof.
+    todo "universes"%string.
+  Qed.
+
+  Lemma subst_instance_ind_sort_id Σ mdecl ind idecl : 
+    declared_inductive Σ mdecl ind idecl ->
+    forall (oib : on_ind_body (lift_typing typing) (Σ, ind_universes mdecl)
+    (inductive_mind ind) mdecl (inductive_ind ind) idecl),
+    let u :=  PCUICLookup.abstract_instance (ind_universes mdecl) in
+    subst_instance_univ u (ind_sort oib) = ind_sort oib.
+  Proof.
+    todo "universes"%string.
+  Qed.
+  
+  Lemma subst_instance_ind_type_id Σ mdecl ind idecl : 
+    declared_inductive Σ mdecl ind idecl ->
+    let u :=  PCUICLookup.abstract_instance (ind_universes mdecl) in
+    subst_instance_constr u (ind_type idecl) = ind_type idecl.
+  Proof.
+    todo "universes"%string.
+  Qed.
+
+  Lemma isType_subst_instance_id Σ univs Γ T : 
+    let u :=  PCUICLookup.abstract_instance univs in
+    isType (Σ, univs) Γ T -> subst_instance_constr u T = T.
+  Proof.
+    todo "universes"%string.
+  Qed.
 
   (* Well, it's a smash_context mess! *)
-  Lemma declared_projection {Σ : global_env_ext} {mdecl idecl p pdecl} : 
-    wf Σ.1 ->
-    declared_projection Σ.1 mdecl idecl p pdecl ->
+  Lemma declared_projections {Σ : global_env_ext} {mdecl ind idecl} : 
+    forall (wfΣ : wf Σ.1) (Hdecl : declared_inductive Σ mdecl ind idecl),
+    let oib := declared_inductive_inv weaken_env_prop_typing wfΣ wfΣ Hdecl in
     let u := PCUICLookup.abstract_instance (ind_universes mdecl) in
-    let ind := p.1.1 in
-    isType (Σ.1, ind_universes mdecl)
-      ((vass nAnon (mkApps (tInd ind u) (to_extended_list (smash_context [] (ind_params mdecl)))))::
-         smash_context [] (ind_params mdecl)) pdecl.2.
+    match ind_cshapes oib return Type with
+    | [cs] => 
+      on_projections mdecl (inductive_mind ind) (inductive_ind ind) 
+        idecl (ind_indices oib) cs -> 
+      Alli (fun i pdecl => 
+      isType (Σ.1, ind_universes mdecl)
+        ((vass nAnon (mkApps (tInd ind u) 
+              (to_extended_list (smash_context [] (ind_params mdecl)))))::
+           smash_context [] (ind_params mdecl)) pdecl.2 * 
+        ∑ decl, 
+          (nth_error (smash_context [] (cshape_args cs)) 
+            (context_assumptions (cshape_args cs) - S i) = Some decl) *
+          (projection_type mdecl ind i decl.(decl_type) = pdecl.2) *
+          (projection_type mdecl ind i decl.(decl_type) = 
+             projection_type' mdecl ind  i decl.(decl_type)))%type
+        0 (ind_projs idecl)
+    | _ => True
+    end.
   Proof.
-    intros wfΣ isdecl u ind.
+    intros wfΣ decli oib u.
+    destruct (ind_cshapes oib) as [|? []] eqn:Heq; try contradiction; auto.
+    intros onps.
+    eapply forall_nth_error_Alli.
+    set (eos := CoreTactics.the_end_of_the_section).
+    intros i. Subterm.rec_wf_rel IH i lt. clear eos.
+    rename pr1 into i. simpl; clear H0.
+    set (p := ((ind, ind_npars mdecl), i)).
+    intros pdecl Hp. simpl.
+    set(isdecl := (conj decli (conj Hp eq_refl)) :
+       declared_projection Σ.1 mdecl idecl p pdecl).
     destruct (on_declared_projection wfΣ isdecl) as [oni onp].
-    set (declared_inductive_inv _ wfΣ _ isdecl.p1) as oib in *.
-    clearbody oib.
-    have onpars := onParams _ _ _ _ (declared_minductive_inv weaken_env_prop_typing wfΣ wfΣ isdecl.p1.p1).
-    have parslen := onNpars _ _ _ _ (declared_minductive_inv weaken_env_prop_typing wfΣ wfΣ isdecl.p1.p1).
-    simpl in onp. destruct (ind_cshapes oib) as [|? []] eqn:Heq; try contradiction.
+    set (declared_inductive_inv _ _ _ _) as oib' in onp.
+    change oib' with oib in *. clear oib'.
+    simpl in oib.
+    have onpars := onParams _ _ _ _ 
+      (declared_minductive_inv weaken_env_prop_typing wfΣ wfΣ decli.p1).
+    have parslen := onNpars _ _ _ _ 
+      (declared_minductive_inv weaken_env_prop_typing wfΣ wfΣ decli.p1).
+    simpl in onp. rewrite Heq in onp. 
+    destruct onp as [[[wfargs onProjs] Hp2] onp].
     red in onp.
     destruct (nth_error (smash_context [] _) _) eqn:Heq'; try contradiction.
+    destruct onp as [onna onp].
     rewrite {}onp.
-    assert(onProjs :  on_projections mdecl (inductive_mind p.1.1) (inductive_ind p.1.1) idecl (ind_indices oib) c).
-    { destruct oib.
-      assert (ind_projs idecl <> []).
-      { destruct isdecl as [? [hnth]]. eapply nth_error_Some_non_nil in hnth; auto. }
-      simpl in Heq. simpl. rewrite Heq in onProjections.
-      now specialize (onProjections H). }
+    apply on_projections_decl in onps.
+    clearbody oib.
     assert(projslen : #|ind_projs idecl| = (context_assumptions (cshape_args c))).
     { now destruct onProjs. }
     assert (some_proj :#|ind_projs idecl| > 0).
     { destruct isdecl as [ [] []]. now apply nth_error_Some_length in H1. }
-    pose proof (onConstructors oib) as onc. 
-    red in onc. rewrite Heq in onc. inv onc. clear X0.
-    eapply on_cargs in X.
     simpl.
-    assert (wf_local (Σ.1, ind_universes mdecl) (arities_context (ind_bodies mdecl))).
+    assert (wfarities : wf_local (Σ.1, ind_universes mdecl)
+       (arities_context (ind_bodies mdecl))).
     { eapply wf_arities_context; eauto. now destruct isdecl as [[] ?]. }
-    eapply PCUICClosed.type_local_ctx_All_local_env in X.
+    eapply PCUICClosed.type_local_ctx_All_local_env in wfargs.
     2:{ eapply All_local_env_app_inv. split; auto.
         red in onpars. eapply (All_local_env_impl _ _ _ onpars).
         intros. destruct T; simpl in *.
         - eapply weaken_ctx; auto.
-        - destruct X1 as [s Hs]. exists s. apply weaken_ctx; auto. }
+        - destruct X as [s Hs]. exists s. apply weaken_ctx; auto. }
+    pose proof wfargs as X.
     rewrite -(app_context_nil_l (arities_context _)) in X.
     rewrite -app_context_assoc in X.
     eapply (substitution_wf_local _ []) in X; auto.
-    2:{ eapply subslet_inds_gen; eauto. destruct isdecl as []; eauto. }
+    2:{ eapply subslet_inds_gen; eauto. }
     rewrite app_context_nil_l in X.
-    epose proof (nth_error_subst_context _ _ _ _).
-    erewrite Heq' in H. autorewrite with len in H. clear Heq'.
-    rewrite subst_context_smash_context in H.
-    autorewrite with len in H. rewrite subst_context_nil in H.
     move: X.
     rewrite subst_context_app.
     rewrite (closed_ctx_subst _ _ (ind_params mdecl)).
     red in onpars. eapply closed_wf_local; [|eauto]. auto.
-    assert (parsu : subst_instance_context u (ind_params mdecl) = ind_params mdecl). admit.
-    assert (sortu : subst_instance_univ u (ind_sort oib) = ind_sort oib). admit.
+    assert (parsu : subst_instance_context u (ind_params mdecl) = ind_params mdecl). 
+    { red in onpars. eapply subst_instance_context_id. eauto. }
+    assert (sortu : subst_instance_univ u (ind_sort oib) = ind_sort oib).
+    { apply subst_instance_ind_sort_id; eauto. }
     pose proof (spine_subst_to_extended_list_k (Σ.1, ind_universes mdecl)
       (ind_params mdecl) []).
     forward X; auto.
@@ -745,33 +1056,40 @@ Section Validity.
     rewrite app_context_nil_l in X.
     rewrite closed_ctx_lift in X.
     red in onpars. eapply closed_wf_local; [|eauto]. auto.
-    assert(wf_local (Σ.1, ind_universes mdecl) (ind_params mdecl ,, vass nAnon (mkApps (tInd ind u) (to_extended_list (ind_params mdecl))))).
-    constructor. auto. red. exists (ind_sort oib).
-    eapply type_mkApps. econstructor; eauto.
-    destruct isdecl as []; eauto. subst u. admit.
-    rewrite (ind_arity_eq oib).
-    rewrite subst_instance_constr_it_mkProd_or_LetIn.
-    rewrite -(app_nil_r (to_extended_list _)).
-    eapply typing_spine_it_mkProd_or_LetIn'; auto.
-    rewrite parsu. eapply X.
-    constructor. left. eexists _, _; simpl; intuition auto.
-    pose proof (onProjs.(on_projs_noidx _ _ _ _ _ _)).
-    destruct (ind_indices oib); simpl in H0; try discriminate.
-    simpl. rewrite sortu. reflexivity.
-    rewrite -subst_instance_constr_it_mkProd_or_LetIn.
-    right. pose proof (onArity oib). rewrite -(oib.(ind_arity_eq)).
-    destruct X1 as [s Hs]. exists s.
-    eapply (weaken_ctx (Γ:=[])). auto. auto. admit.
+    assert(wf_local (Σ.1, ind_universes mdecl) (ind_params mdecl ,,
+       vass nAnon (mkApps (tInd ind u) (to_extended_list (ind_params mdecl))))).
+    { constructor. auto. red. exists (ind_sort oib).
+      eapply type_mkApps. econstructor; eauto.
+      destruct isdecl as []; eauto. subst u.
+      eapply consistent_instance_ext_abstract_instance. 2:destruct decli; eauto. 
+      now auto.
+      rewrite (ind_arity_eq oib).
+      rewrite subst_instance_constr_it_mkProd_or_LetIn.
+      rewrite -(app_nil_r (to_extended_list _)).
+      eapply typing_spine_it_mkProd_or_LetIn'; auto.
+      rewrite parsu. eapply X.
+      constructor. left. eexists _, _; simpl; intuition auto.
+      simpl in oib.
+      pose proof (onProjs.(on_projs_noidx _ _ _ _ _ _)).
+      destruct (ind_indices oib); simpl in H; try discriminate.
+      simpl. rewrite sortu. reflexivity.
+      rewrite -subst_instance_constr_it_mkProd_or_LetIn.
+      right. pose proof (onArity oib). rewrite -(oib.(ind_arity_eq)).
+      destruct X0 as [s Hs]. exists s.
+      eapply (weaken_ctx (Γ:=[])); auto.
+      rewrite (subst_instance_ind_type_id Σ.1 _ ind); auto. }
     intros wf.
-    generalize (weakening_wf_local _ _ _ [_] _ wf X1).
-    simpl; clear X1 wf.
+    generalize (weakening_wf_local _ _ _ [_] _ wf X0).
+    simpl; clear X0 wf.
     move/wf_local_smash_context => /=.
     rewrite smash_context_app /= smash_context_acc.
-    red in onpars. eapply closed_wf_local; [|eauto]. auto.
-    set(indsubst := (inds (inductive_mind p.1.1) (PCUICLookup.abstract_instance (PCUICEnvironment.ind_universes mdecl))
+
+    set(indsubst := (inds (inductive_mind ind) 
+      (PCUICLookup.abstract_instance (PCUICEnvironment.ind_universes mdecl))
       (PCUICEnvironment.ind_bodies mdecl))) in *.
-    set (projsubst :=  (projs {| inductive_mind := inductive_mind p.1.1; inductive_ind := inductive_ind p.1.1 |}
-    (PCUICEnvironment.ind_npars mdecl) p.2)) in *.
+    set (projsubst :=  (projs {| inductive_mind := inductive_mind ind; 
+       inductive_ind := inductive_ind ind |}
+      (PCUICEnvironment.ind_npars mdecl) i)) in *.
     rewrite lift_context_app. simpl.
     rewrite [subst_context _ _ (_ ++ _)]subst_context_app.
     simpl. unfold app_context. simpl.
@@ -782,83 +1100,383 @@ Section Validity.
     rewrite extended_subst_to_extended_list_k.
     fold (to_extended_list (smash_context [] (ind_params mdecl))).
     intros wfl.
-    rewrite PCUICClosed.closed_ctx_lift in wfl. admit.
-    
+    rewrite PCUICClosed.closed_ctx_lift in wfl.
+    { eapply closedn_smash_context.
+      eapply closed_wf_local in wfargs; auto.
+      rewrite closedn_ctx_app in wfargs.
+      simpl in wfargs; autorewrite with len in wfargs.
+      move/andP: wfargs => [_ clargs].
+      clear -isdecl wfΣ clargs.
+      eapply (closedn_ctx_lift 1).
+      rewrite Nat.add_0_r.
+      eapply (closedn_ctx_subst 0 #|ind_params mdecl|).
+      now unfold indsubst; rewrite inds_length.
+      unfold indsubst.
+      eapply declared_minductive_closed_inds.
+      2:destruct isdecl as [ [] ?]; eauto. eauto. } 
+    rewrite -app_assoc in wfl.
+    apply All_local_env_app in wfl as [wfctx wfsargs].
+    rewrite smash_context_app in Heq'.
+    rewrite smash_context_acc in Heq'. 
+    rewrite nth_error_app_lt in Heq'.
+    autorewrite with len. lia.
+    set (idx := context_assumptions (cshape_args c) - S i) in *.
+    unshelve epose proof (nth_error_All_local_env (n:=idx) _ wfsargs).
+    autorewrite with len. rewrite /lift_context /subst_context !context_assumptions_fold.
+    subst idx; lia.
+    destruct (nth_error (subst_context _ 1 _) idx) as [c1|] eqn:hidx.
+    simpl in X0. unfold on_local_decl in X0.
+    assert(decl_body c1 = None).
+    { apply nth_error_assumption_context in hidx; auto.
+      rewrite /subst_context /lift_context.
+      apply assumption_context_fold, smash_context_assumption_context. constructor. }
+    rewrite H in X0. 2:{ simpl in X0; contradiction. }
+    destruct X0 as [s Hs].
+    eapply (substitution (Σ.1, ind_universes mdecl) (_ :: _) (skipn _ _) projsubst []) 
+      in Hs; auto.
+    simpl in Hs.
+    rewrite nth_error_subst_context in Heq'.
+    autorewrite with len in Heq'. simpl in Heq'.
+    epose proof (nth_error_lift_context_eq _ (smash_context [] (ind_params mdecl))).
+    autorewrite with len in H0.
+    erewrite H0 in Heq'. simpl in Heq'. clear H0.
+    rewrite !option_map_two in Heq'.
+    apply option_map_Some in Heq' as [arg [nthidx eq]].
+    rewrite nth_error_subst_context in hidx.
+    autorewrite with len in hidx. simpl in hidx.
+    rewrite (smash_context_lift []) in hidx.
+    rewrite (smash_context_subst []) in hidx.
+    rewrite (nth_error_lift_context_eq _ [vass nAnon (mkApps (tInd ind u)  [])]) in hidx.
+    simpl in hidx. autorewrite with len in hidx.
+    rewrite nth_error_subst_context in hidx. autorewrite with len in hidx.
+    simpl in hidx.
+    rewrite !option_map_two in hidx.
+    assert(clarg : closedn (i + #|ind_params mdecl| + #|ind_bodies mdecl|) (decl_type arg)).
+    { assert(wf_local (Σ.1, ind_universes mdecl)
+       (arities_context (ind_bodies mdecl) ,,, ind_params mdecl ,,, 
+        smash_context [] (cshape_args c))).
+      apply All_local_env_app_inv; split; auto.
+      now apply All_local_env_app in wfargs as [wfindpars wfargs].
+      apply wf_local_rel_smash_context; auto.
+      eapply closed_wf_local in X0; auto.
+      eapply (closed_ctx_decl (n:=idx)) in X0; eauto.
+      2:{ rewrite nth_error_app_lt. autorewrite with len. simpl; lia.
+          now eapply nthidx. }
+      move/andP: X0 => [_ clty]. 
+      eapply closed_upwards; eauto.
+      autorewrite with len; simpl. simpl in idx. lia. }
+    rewrite nthidx in hidx. simpl in hidx. noconf hidx. simpl in *.
+    subst c0.
+    destruct ind as [mind ind]; simpl in *.
+    autorewrite with len. simpl.
+    revert Hs.
+    assert(context_assumptions (cshape_args c) - S idx = i) as -> by lia.
+    rewrite !context_assumptions_fold.
+    assert(context_assumptions (cshape_args c) - S idx + 1 = S i) as -> by lia.
+    intros Hs.
+    assert (projection_type mdecl {| inductive_mind := mind; inductive_ind := ind |}
+       i (decl_type arg) = 
+      projection_type' mdecl {| inductive_mind := mind; inductive_ind := ind |} i
+         (decl_type arg)).
+    { eapply nth_error_Some_length in nthidx.
+      autorewrite with len in nthidx. simpl in nthidx.
+      unfold projection_type, projection_type'. simpl.
+      fold indsubst projsubst.
+      rewrite distr_subst.
+      f_equal. 
+      { clear. subst projsubst. induction i; simpl; auto.
+        f_equal. auto. }
+      rewrite /projsubst projs_length.
+      replace (context_assumptions (cshape_args c) - S idx + 1) with
+      (context_assumptions (cshape_args c) - idx) by lia.
+      simpl in idx.
+      epose proof (commut_lift_subst_rec _ _ 1 (i + ind_npars mdecl) i).
+      rewrite -Nat.add_1_r Nat.add_assoc. erewrite <-H0. 2:lia.
+      clear H0.
+      epose proof (commut_lift_subst_rec _ _ 1 i i) as hs.
+      rewrite Nat.add_1_r in hs. rewrite <- hs; try lia. clear hs. f_equal.
+      rewrite distr_subst_rec.
+      clear H.
+      rewrite map_subst_closedn.
+      rewrite -parslen.
+      eapply closedn_extended_subst. eapply closed_wf_local. 2:eauto. auto.
+      f_equal. autorewrite with len.
+      epose proof (commut_lift_subst_rec _ _ (ind_npars mdecl) (i + #|ind_params mdecl|) 
+        (i + #|ind_params mdecl|)) as hs.
+      rewrite parslen. erewrite <-hs. 2:lia.
+      rewrite lift_closed; auto.
+      apply (closedn_subst _ 0). 
+      unfold indsubst.
+      eapply (declared_minductive_closed_inds _ {| inductive_mind := mind; 
+                            inductive_ind := ind |}). 
+      2:destruct isdecl as [[] ?]; eauto. auto.
+      simpl. eapply subject_closed in Hs.
+      now rewrite /indsubst inds_length. auto. }
+    split.
+    unfold projection_type in H0.
+    rewrite H0. exists s; auto.
+    exists arg. intuition auto.
 
-
-    rewrite -reln_lift.
-    set(foo:= subst_context _ _ _).
-    rewrite subst_context_app.
-    eapply nth_error_All_local_env in X.
-    2:{ eapply nth_error_Some_length in H. apply H. }
-    unfold app_context in X. erewrite H in X.
-    simpl in X, H. red in X.
-    destruct c0 as [? [] ?]; simpl in *.
-    unfold subst_decl, map_decl in H; simpl in H.
-    eapply nth_error_smash_context in H. simpl in H. discriminate.
-    clear H.
-    intros. rewrite nth_error_nil // in H.
-    destruct X as [s Hs].
-    rewrite smash_context_length /= in Hs.
-    rewrite PCUICClosed.context_assumptions_app Nat.add_0_r in Hs.
-    clear H.
-    set (k := context_assumptions (cshape_args c) - p.2) in *.
-    rewrite subst_context_app Nat.add_0_r in Hs.
-    rewrite (closed_ctx_subst _ _ (ind_params mdecl)) in Hs.
-    red in onpars. eapply closed_wf_local; [|eauto]. auto.
-    rewrite /app_context smash_context_app in Hs.
-    exists s. red.
-    rewrite smash_context_acc in Hs.
-    rewrite skipn_app in Hs.
-    autorewrite with len in Hs. rewrite !smash_context_length in Hs.
-    rewrite context_assumptions_fold in Hs.
-    rewrite (skipn_0_eq _ (S _ - _)) in Hs.
-    simpl length. lia.
-    destruct isdecl as [? []]. apply nth_error_Some_length in H0.
-    rewrite projslen in H0. rewrite projslen in some_proj. lia.
+    unfold projsubst. clear Hs.
+    clear -wfΣ parslen onps projslen some_proj IH Hp2 decli.
+    rewrite (smash_context_lift []).
+    rewrite (smash_context_subst []).
+    rewrite -(firstn_skipn (S idx) (smash_context [] (cshape_args c))).
+    rewrite subst_context_app lift_context_app subst_context_app.
+    autorewrite with len.
+    rewrite skipn_all_app_eq.
+    autorewrite with len.
+    rewrite firstn_length_le; auto. rewrite smash_context_length.
     simpl. lia.
+    induction i. subst idx.
+    - assert (S (context_assumptions (cshape_args c) - 1) =
+       (context_assumptions (cshape_args c))) as -> by lia.
+      rewrite skipn_all2.
+      autorewrite with len; simpl; auto.
+      constructor.
+    - forward IHi.
+      intros. eapply (IH i0). lia. auto. 
+      forward IHi by lia. simpl in IHi.
+      subst idx.
+      destruct (skipn (S (context_assumptions (cshape_args c) - S (S i))) 
+        (smash_context [] (cshape_args c))) eqn:eqargs.
+      apply (f_equal (@length _)) in eqargs.
+      autorewrite with len in eqargs.
+      rewrite skipn_length in eqargs. autorewrite with len. simpl; lia.
+      autorewrite with len in eqargs. simpl in eqargs. lia.
+      rewrite subst_context_snoc lift_context_snoc subst_context_snoc.
+      simpl.
+      destruct c0 as [? [] ?].
+      * simpl in eqargs.
+        pose proof (@smash_context_assumption_context [] (cshape_args c)).
+        forward H by constructor.
+        eapply assumption_context_skipn in H.
+        rewrite -> eqargs in H. elimtype False; inv H.
+      * apply skipn_eq_cons in eqargs as [Hnth eqargs].
+        constructor.
+        + replace (S (S (context_assumptions (cshape_args c) - S (S i)))) 
+            with (S (context_assumptions (cshape_args c) - S i)) in eqargs by lia.
+          rewrite eqargs in IHi. apply IHi.
+        + set substdecl := (subst
+             (inds (inductive_mind ind) u (ind_bodies mdecl)) (S (ind_npars mdecl))
+            (subst (projs ind (ind_npars mdecl) i) 0
+              (lift 1 i decl_type))).
+          specialize (IH i ltac:(lia)).
+          autorewrite with len.
+          eapply (f_equal (@length _)) in eqargs.
+          rewrite skipn_length in eqargs.
+          autorewrite with len. simpl; lia.
+          autorewrite with len in eqargs. simpl in eqargs.
+          eapply nth_error_alli in onps; eauto. simpl in onps.
+          destruct onps as [pdecl Hnth'].
+          replace ((context_assumptions (cshape_args c) - 
+            S (S (context_assumptions (cshape_args c) - S (S i)))))
+            with i in eqargs, Hnth' by lia. rewrite -eqargs.
+          rewrite /lift_decl /subst_decl. simpl.
+          autorewrite with len.
+          epose proof (commut_lift_subst_rec _ _ 1 (i + #|ind_params mdecl|) i).
+          erewrite H. 2:lia. clear H.
+          specialize (IH _ Hnth').
 
-
-    
-
-
-
-    replace ((context_assumptions (cshape_args c) +
-    context_assumptions (PCUICEnvironment.ind_params mdecl) -
-    S (PCUICEnvironment.context_assumptions (cshape_args c) - p.2)))
-    with  (context_assumptions (PCUICEnvironment.ind_params mdecl) + S p.2) by lia.
-        S (PCUICEnvironment.context_assumptions (cshape_args c) - p.2)))
-    autorewrite with len in Hs.
-
-    eexists _.
-    rename X into args.
-    apply type_local_ctx_Pclosed in args.
-    red in onpars.
-    eapply All_local_env_Pclosed in onpars.
-    eapply (Alli_impl (Q:=fun i d => closed_decl (#|ind_params mdecl| + i + #|arities_context (ind_bodies mdecl)|) d)) in args.
-    2:{ intros n x. rewrite app_context_length. 
-        intros H; eapply closed_decl_upwards; eauto. lia. }
-    eapply (Alli_shiftn (P:=fun i d => closed_decl (i + #|arities_context (ind_bodies mdecl)|) d)) in args.
-    rewrite Nat.add_0_r in args.
-    eapply (Alli_impl (Q:=fun i d => closed_decl (i + #|arities_context (ind_bodies mdecl)|) d)) in onpars.
-    2:{ intros n x d. eapply closed_decl_upwards; eauto; lia. }
-    epose proof (Alli_app_inv onpars). rewrite List.rev_length /= in X.
-    specialize (X args). rewrite -List.rev_app_distr in X.
-    clear onpars args.
-    eapply (Alli_impl (Q:=fun i d => closed_decl (#|arities_context (ind_bodies mdecl)| + i) d)) in X.
-    2:intros; eapply closed_decl_upwards; eauto; lia.
-    eapply closed_smash_context in X.
-    eapply Alli_rev_nth_error in X; eauto.
-    rewrite smash_context_length in X. simpl in X.
-    eapply nth_error_Some_length in Heq'. rewrite smash_context_length in Heq'.
-    simpl in Heq'. unfold closed_decl in X.
-    move/andP: X => [] _ cl.
-    eapply closed_upwards. eauto. rewrite arities_context_length.
-    rewrite context_assumptions_app parslen.
-    rewrite context_assumptions_app in Heq'. lia.
+          eapply meta_conv. econstructor.
+          split; eauto. simpl.
+          eapply meta_conv. econstructor.
+          destruct IH as [[s isTy] _].
+          now eapply typing_wf_local in isTy.
+          simpl. reflexivity. simpl.
+          rewrite lift_mkApps. simpl. destruct ind; simpl.
+          reflexivity. autorewrite with len.
+          simpl. 
+          rewrite context_assumptions_smash_context /= //.
+          assert(subst_instance_constr u pdecl.2 = pdecl.2) as ->.
+          { eapply isType_subst_instance_id. apply IH. }
+          destruct IH as [isTy [decl [[nthdecl eqpdecl] ptyeq]]].
+          move ptyeq at bottom. 
+          replace  (S (context_assumptions (cshape_args c) - S (S i))) with 
+           (context_assumptions (cshape_args c) - S i) in Hnth by lia.
+          rewrite nthdecl in Hnth. noconf Hnth. simpl in ptyeq.
+          rewrite -eqpdecl. simpl.
+          rewrite ptyeq. unfold projection_type'.
+          fold indsubst. destruct ind as [mind ind]; simpl in *.
+          set (projsubst := projs {| inductive_mind := mind; inductive_ind := ind |} (ind_npars mdecl) i) in *.
+          rewrite -eqpdecl in isTy.
+          eapply isType_closed in isTy.
+          simpl in isTy. autorewrite with len in isTy. simpl in isTy.
+          rewrite ptyeq in isTy.
+          unfold projection_type' in isTy.
+          epose proof (commut_lift_subst_rec _ _ 1 (i + #|ind_params mdecl|) i).
+          erewrite H in isTy by lia.
+          rewrite H; try lia.
+          rewrite (subst_id _ (({|
+            decl_name := nAnon;
+            decl_body := None;
+            decl_type := mkApps
+                          (tInd
+                              {| inductive_mind := mind; inductive_ind := ind |}
+                              u)
+                          (to_extended_list
+                              (smash_context [] (ind_params mdecl))) |}
+            :: smash_context [] (ind_params mdecl)))).
+          ++ simpl. autorewrite with len.
+            rewrite context_assumptions_smash_context //.                            
+          ++ constructor. apply smash_context_assumption_context; constructor.
+          ++ unfold to_extended_list, to_extended_list_k.  simpl.
+            rewrite -reln_lift /= (reln_acc [_]) rev_app_distr /= //.
+          ++ now rewrite (Nat.add_1_r i).
+          ++ simpl. auto.
   Qed.
- *)
 
+  Lemma declared_projection_type {Σ : global_env_ext} {mdecl idecl p pdecl} : 
+    wf Σ.1 ->
+    declared_projection Σ mdecl idecl p pdecl ->
+    let u := PCUICLookup.abstract_instance (ind_universes mdecl) in    
+    isType (Σ.1, ind_universes mdecl)
+      ((vass nAnon (mkApps (tInd p.1.1 u) 
+            (to_extended_list (smash_context [] (ind_params mdecl)))))::
+         smash_context [] (ind_params mdecl)) pdecl.2.
+  Proof.
+    intros wfΣ declp.
+    destruct (on_declared_projection wfΣ declp) as [oni onp].
+    specialize (declared_projections wfΣ (let (x, _) := declp in x)).
+    set(oib := declared_inductive_inv _ _ _ _) in *.
+    intros onprojs u.
+    clearbody oib.
+    simpl in *.
+    destruct (ind_cshapes oib) as [|? []]; try contradiction.
+    forward onprojs. intuition auto.
+    destruct declp as [decli [Hnth Hpars]].
+    eapply nth_error_alli in onprojs; eauto.
+    simpl in onprojs. intuition auto.
+  Qed.
+
+  Lemma subst_instance_subst_context u s k Γ : 
+    subst_instance_context u (subst_context s k Γ) =
+    subst_context (map (subst_instance_constr u) s) k (subst_instance_context u Γ).
+  Proof.
+    rewrite /subst_instance_context /map_context !subst_context_alt.
+    rewrite map_mapi mapi_map. apply mapi_rec_ext.
+    intros. rewrite /subst_decl !PCUICAstUtils.compose_map_decl.
+    apply PCUICAstUtils.map_decl_ext => ?.
+    rewrite map_length. now rewrite subst_subst_instance_constr.
+  Qed.
+
+  Lemma subst_instance_context_smash u Γ Δ : 
+    subst_instance_context u (smash_context Δ Γ) = 
+    smash_context (subst_instance_context u Δ) (subst_instance_context u Γ).
+  Proof.
+    induction Γ as [|[? [] ?] ?] in Δ |- *; simpl; auto.
+    - rewrite IHΓ. f_equal.
+      now rewrite subst_instance_subst_context.
+    - rewrite IHΓ subst_instance_context_app /= //.
+  Qed.
+
+  Lemma map_inst_idsn l l' n :
+    #|l| = n ->
+    map (inst (l ⋅n l')) (idsn n) = l.
+  Proof.
+    induction n in l, l' |- *.
+    - destruct l => //.
+    - destruct l as [|l a] using rev_case => // /=.
+      rewrite app_length /= Nat.add_1_r => [=].
+      intros; subst n.
+      simpl. rewrite map_app.
+      f_equal. rewrite subst_consn_app.
+      now apply IHn.
+      simpl.
+      destruct (subst_consn_lt #|l| (l ++ [a]) l') as [a' [hnth heq]].
+      rewrite app_length. simpl; lia.
+      rewrite heq. rewrite nth_error_app_ge in hnth; auto.
+      rewrite Nat.sub_diag in hnth. simpl in hnth. congruence.
+  Qed.
+  
+  Lemma context_subst_extended_subst Γ args s : 
+    context_subst Γ args s ->
+    s = map (inst (List.rev args ⋅n ids)) (extended_subst Γ 0).
+  Proof.
+    induction 1.
+    - simpl; auto.
+    - simpl.
+      rewrite lift_extended_subst.
+      rewrite map_map_compose.
+      rewrite List.rev_app_distr. simpl. f_equal.
+      rewrite IHX. apply map_ext.
+      intros. autorewrite with sigma.
+      apply inst_ext.
+      rewrite subst_consn_subst_cons.
+      now rewrite subst_cons_shift.
+    - simpl.
+      f_equal; auto.
+      rewrite IHX.
+      autorewrite with sigma.
+      apply inst_ext.
+      rewrite ren_lift_renaming. autorewrite with len.
+      rewrite subst_consn_compose.
+      autorewrite with sigma.
+      unfold Upn.
+      rewrite subst_consn_compose.
+      apply subst_consn_proper; first last.
+      rewrite -subst_consn_app.
+      rewrite shiftk_compose.
+      rewrite subst_consn_shiftn //.
+      autorewrite with len. now rewrite (context_subst_length2 X).
+      rewrite map_inst_idsn //. now autorewrite with len.
+  Qed.
+
+  Lemma spine_subst_smash {Σ Γ inst s Δ} : 
+    wf Σ.1 ->
+    spine_subst Σ Γ inst s Δ ->
+    spine_subst Σ Γ inst (List.rev inst) (smash_context [] Δ).
+  Proof.
+    intros wfΣ [].
+    assert (context_subst (smash_context [] Δ) inst (List.rev inst)).
+    { apply closed_wf_local in spine_dom_wf.
+      clear -inst_ctx_subst spine_dom_wf. induction inst_ctx_subst.
+      constructor. rewrite List.rev_app_distr /=.
+      rewrite smash_context_acc. simpl.
+      constructor. auto.
+      simpl. rewrite smash_context_acc. simpl. auto.
+      auto. }
+    split; auto.
+    - eapply All_local_env_app_inv; split; auto.
+      eapply wf_local_rel_smash_context; auto.
+    - induction inst_subslet in inst, inst_ctx_subst, spine_codom_wf |- *.
+      depelim inst_ctx_subst.
+      + constructor.
+      + depelim inst_ctx_subst; simpl in H; noconf H.
+        simpl. rewrite smash_context_acc.
+        simpl. rewrite List.rev_app_distr.
+        depelim spine_codom_wf; simpl in H; noconf H.
+        constructor. now apply IHinst_subslet.
+        eapply meta_conv. eauto.
+        simpl.
+        autorewrite with sigma.
+        apply inst_ext. rewrite ren_lift_renaming.
+        autorewrite with sigma.
+        unfold Upn. rewrite subst_consn_compose.
+        autorewrite with sigma.
+        apply subst_consn_proper.
+        2:{ rewrite -(subst_compose_assoc (↑^#|Δ|)).
+            rewrite subst_consn_shiftn.
+            2:now autorewrite with len.
+            autorewrite with sigma.
+            rewrite subst_consn_shiftn //.
+            rewrite List.rev_length.
+            now apply context_subst_length2 in inst_ctx_subst. }
+        clear -inst_ctx_subst.
+        rewrite subst_consn_compose.
+        rewrite map_inst_idsn. now autorewrite with len.
+        now apply context_subst_extended_subst.
+      + simpl. rewrite smash_context_acc.
+        simpl. depelim spine_codom_wf; simpl in H; noconf H.
+        depelim inst_ctx_subst; simpl in H; noconf H; simpl in H0; noconf H0.
+        apply IHinst_subslet; auto.
+  Qed.
+
+  Lemma subst_instance_instance_id u mdecl : 
+    subst_instance_instance u (PCUICLookup.abstract_instance (ind_universes mdecl)) = u.
+  Proof.
+    todo "universes"%string.
+  Qed.
 
   Theorem validity :
     env_prop (fun Σ Γ t T => isWfArity_or_Type Σ Γ T)
@@ -870,7 +1488,7 @@ Section Validity.
   Proof.
     apply typing_ind_env; intros; rename_all_hyps.
 
-    - auto. 
+    - auto.
 
     - destruct (nth_error_All_local_env_over heq_nth_error X) as [HΓ' Hd].
       destruct decl as [na [b|] ty]; cbn -[skipn] in *.
@@ -1030,15 +1648,33 @@ Section Validity.
 
     - (* Proj *)
       right.
-      destruct (on_declared_projection wf isdecl) as [oni onp].
-      destruct declared_inductive_inv. simpl in onp.
-      as [[onm oni] onp]=> //.
-      destruct onp as [s Hty].
-      exists s.
+      pose proof isdecl as isdecl'.
+      eapply declared_projection_type in isdecl'; eauto.
       subst ty.
-      (* eapply typing_subst_instance in Hty. *)
-      todo "projection"%string.
-
+      destruct isdecl' as [s Hs].
+      unshelve eapply isWAT_mkApps_Ind in X2 as [parsubst [argsubst [[sppar sparg] cu]]]; eauto.
+      eapply isdecl.p1.
+      eapply (typing_subst_instance_decl _ _ _ _ _ _ _ wf isdecl.p1.p1) in Hs; eauto.
+      simpl in Hs.
+      exists (subst_instance_univ u s).
+      unfold PCUICTypingDef.typing in *.
+      eapply (weaken_ctx Γ) in Hs; eauto.
+      rewrite -heq_length in sppar. rewrite firstn_all in sppar.
+      rewrite subst_instance_context_smash in Hs. simpl in Hs.
+      eapply spine_subst_smash in sppar => //.
+      eapply (substitution _ Γ _ _ [_] _ _ wf sppar) in Hs.
+      simpl in Hs.
+      eapply (substitution _ Γ [_] [c] [] _ _ wf) in Hs.
+      simpl in Hs. rewrite (subst_app_simpl [_]) /= //.
+      constructor. constructor.
+      simpl. rewrite subst_empty.
+      rewrite subst_instance_constr_mkApps subst_mkApps /=.
+      rewrite subst_instance_instance_id.
+      rewrite subst_instance_to_extended_list.
+      rewrite subst_instance_context_smash.
+      rewrite (spine_subst_subst_to_extended_list_k sppar).
+      assumption.
+      
     - (* Fix *)
       eapply nth_error_all in X0; eauto.
       firstorder auto.
