erasure/theories/EArities.v
@@ -35,13 +35,13 @@ Lemma isArity_ind_type (Σ : global_env_ext) mind ind idecl :
   declared_inductive (fst Σ) mind ind idecl ->
   isArity (ind_type idecl).
 Proof.
-  intros. eapply PCUICWeakeningEnv.declared_inductive_inv with (P := typing) in H; eauto.
+  intros. 
+  eapply (PCUICWeakeningEnv.declared_inductive_inv PCUICWeakeningEnv.weaken_env_prop_typing) in H; eauto.
   - inv H. rewrite ind_arity_eq.
     change PCUICEnvironment.it_mkProd_or_LetIn with it_mkProd_or_LetIn.
     rewrite <- it_mkProd_or_LetIn_app.
     clear.
     eapply it_mkProd_isArity. econstructor.
-  - eapply PCUICWeakeningEnv.weaken_env_prop_typing.
 Qed.
 
 Lemma isWfArity_prod_inv:
@@ -232,9 +232,9 @@ Proof.
     (* eapply isArity_typing_spine_inv in t0; eauto. *)
     (* destruct t0 as (? & [] & ?). *)
     (* eapply PCUICCumulativity.red_cumul in X. *)
-    destruct (PCUICWeakeningEnv.on_declared_constructor _ d) as [XX [s [XX1 [Ht [cs XX2]]]]].
+    destruct (PCUICWeakeningEnv.on_declared_constructor _ d) as [XX [s [XX1 Ht]]].
     destruct x5 as [[? ?] ?]; cbn in *; subst.
-    destruct Ht. subst.
+    destruct Ht. unfold cdecl_type in cstr_eq. simpl in cstr_eq. subst.
     change PCUICEnvironment.it_mkProd_or_LetIn with it_mkProd_or_LetIn in c2.
     change PCUICEnvironment.ind_params with ind_params in *.
     change PCUICEnvironment.to_extended_list_k with to_extended_list_k in *.
@@ -246,10 +246,10 @@ Proof.
     cbn in c2.
     rewrite PCUICUnivSubst.subst_instance_context_length in *.
     rewrite app_length in *.
-    destruct (Nat.leb_spec (#|cshape_args| + #|ind_params x3| + 0) (#|ind_bodies x3| - S (inductive_ind ind) + #|ind_params x3| + #|cshape_args|)). 2:lia.
+    destruct (Nat.leb_spec (#|cshape_args s| + #|ind_params x3| + 0) (#|ind_bodies x3| - S (inductive_ind ind) + #|ind_params x3| + #|cshape_args s|)). 2:lia.
     clear H.
     assert ((#|ind_bodies x3| - S (inductive_ind ind) + #|ind_params x3| +
-                                                                         #|cshape_args| - (#|cshape_args| + #|ind_params x3| + 0)) < #|inds (inductive_mind ind) u (ind_bodies x3)|).
+                                                                         #|cshape_args s| - (#|cshape_args s| + #|ind_params x3| + 0)) < #|inds (inductive_mind ind) u (ind_bodies x3)|).
     { rewrite inds_length. lia. }
     eapply nth_error_Some in H.
     destruct (nth_error (inds _ _ _) _) eqn:Heq; try congruence.
