pcuic/theories/PCUICElimination.v
@@ -131,20 +131,20 @@ Proof.
     destruct (Universe.is_small u); try congruence.
 Qed.
 
-Lemma elim_sort_intype {cf:checker_flags} Σ mdecl ind idecl ind_indices ind_sort sorts :
+Lemma elim_sort_intype {cf:checker_flags} Σ mdecl ind idecl ind_indices ind_sort cshapes :
   universe_family ind_sort = InProp ->
-  leb_sort_family InType (elim_sort_prop_ind sorts) ->
+  leb_sort_family InType (elim_sort_prop_ind cshapes) ->
   on_constructors (lift_typing typing)
     (Σ, ind_universes mdecl) mdecl 
     (inductive_ind ind) idecl ind_indices
-    (ind_ctors idecl) sorts ->
+    (ind_ctors idecl) cshapes ->
   (#|ind_ctors idecl| = 0) + 
-  (∑ cdecl sort, 
+  (∑ cdecl cshape, 
     (ind_ctors idecl = [cdecl]) * 
-    (sorts = [sort]) * 
-    (universe_family sort = InProp) *
+    (cshapes = [cshape]) * 
+    (universe_family cshape.(cshape_sort) = InProp) *
     (on_constructor (lift_typing typing) (Σ, ind_universes mdecl) mdecl 
-        (inductive_ind ind) idecl ind_indices cdecl sort))%type.
+        (inductive_ind ind) idecl ind_indices cdecl cshape))%type.
 Proof.
   intros uf lein onc.
   induction onc; simpl in *.
@@ -152,7 +152,7 @@ Proof.
   destruct l' as [|c cs].
   - simpl in *. depelim onc.
     right.
-    destruct (universe_family y) eqn:heq; try discriminate.
+    destruct (universe_family y.(cshape_sort)) eqn:heq; try discriminate.
     eexists; eauto.
   - discriminate.
 Qed.
@@ -349,16 +349,16 @@ Lemma check_ind_sorts_is_prop {cf:checker_flags} (Σ : global_env_ext) mdecl ide
   Universe.is_prop (ind_sort onib) -> 
   check_ind_sorts (lift_typing typing) (Σ.1, ind_universes mdecl)
     (PCUICEnvironment.ind_params mdecl) (PCUICEnvironment.ind_kelim idecl)
-    (ind_indices onib) (ind_ctors_sort onib) (ind_sort onib) ->
-  (#|ind_ctors_sort onib| <= 1) * All Universe.is_prop (ind_ctors_sort onib).
+    (ind_indices onib) (ind_cshapes onib) (ind_sort onib) ->
+  (#|ind_cshapes onib| <= 1) * All (fun cs => Universe.is_prop cs.(cshape_sort)) (ind_cshapes onib).
 Proof.
   intros kelim isp.
   unfold check_ind_sorts, universe_family. simpl.
   rewrite isp. simpl.
-  induction (ind_ctors_sort onib); simpl; auto; try discriminate.
+  induction (ind_cshapes onib); simpl; auto; try discriminate.
   apply not_prop_not_leq_prop in kelim.
   destruct l; simpl in *; try contradiction.
-  destruct (universe_family a) eqn:Heq; try contradiction.
+  destruct (universe_family a.(cshape_sort)) eqn:Heq; try contradiction.
   intros leb.
   apply family_InProp in Heq. now constructor.
 Qed.
@@ -392,7 +392,7 @@ Proof.
   eapply inversion_mkApps in hc as [? [? [hc [hsp hcum]]]]; auto.
   eapply inversion_Construct in hc as [mdecl' [idecl' [cdecl' [wfΓ [declc [cu cum']]]]]]; auto.
   destruct (on_declared_constructor _ declc) as [[oi oib] [cs [Hnth onc]]].
-  set (onib := declared_inductive_inv _ _ _ _ _ _ _ _ _) in *.
+  set (onib := declared_inductive_inv _ _ _ _) in *.
   clearbody onib. clear oib.
   eapply typing_spine_strengthen in hsp; eauto.
   eapply PCUICArities.typing_spine_weaken_concl in hsp; eauto.
@@ -402,7 +402,7 @@ Proof.
   { eapply declared_constructor_valid_ty in declc; eauto. now right. }
   move: X hsp.
   unfold type_of_constructor.
-  rewrite (onc.(cshape).(cshape_eq)).
+  rewrite [cdecl'.1.2](onc.(cstr_eq)).
   rewrite !subst_instance_constr_it_mkProd_or_LetIn !subst_it_mkProd_or_LetIn.
   rewrite - {1}(firstn_skipn (ind_npars mdecl) args).
   rewrite !subst_instance_constr_mkApps.
@@ -430,7 +430,7 @@ Proof.
       apply (consistent_instance_ext_noprop cu).
       eapply leq_universe_prop in l0; intuition eauto. }
     eapply check_ind_sorts_is_prop in X1 as [nctors X1]; eauto.
-    assert(#|ind_ctors_sort onib| = #|ind_ctors idecl|).
+    assert(#|ind_cshapes onib| = #|ind_ctors idecl|).
     clear wat X. clear -onib. pose proof (onib.(onConstructors)).
     eapply All2_length in X. now rewrite X. 
     rewrite H0 in nctors; split; auto.
@@ -458,7 +458,7 @@ Proof.
       (fun Γ Γ' t => 
       ∑ s0 : Universe.t, Σ;;; Γ ,,, Γ' |- t : tSort s0 × Universe.is_prop s0)).
     2:eauto.
-    intros. exists (subst_instance_univ u cs). intuition auto.
+    intros. exists (subst_instance_univ u cs.(cshape_sort)). intuition auto.
     now eapply is_prop_subst_instance.
   * intros _ sp.
     rewrite List.skipn_all2. lia.
@@ -466,7 +466,7 @@ Proof.
     pose proof (onc.(on_cargs)).
     pose proof (onib.(ind_sorts)).
     eapply check_ind_sorts_is_prop in X0 as [nctors X1]; eauto.
-    assert(#|ind_ctors_sort onib| = #|ind_ctors idecl|).
+    assert(#|ind_cshapes onib| = #|ind_ctors idecl|).
     clear -onib. pose proof (onib.(onConstructors)).
     eapply All2_length in X. now rewrite X. now rewrite -H.
     rewrite -it_mkProd_or_LetIn_app in sp.
@@ -529,14 +529,10 @@ Proof.
   pose (d' := d). destruct d' as [? _].
   eapply declared_inductive_inj in H as []; eauto. subst.
   pose proof (declared_projection_projs_nonempty X d).
-  eapply PCUICWeakeningEnv.on_declared_projection in d; eauto.
-  destruct d as (? & ? & ?). destruct p.
-  inv o. inv o0.
-  forward onProjections. eauto.
-  inversion onProjections.
-  clear - on_projs_elim. revert on_projs_elim. generalize (ind_kelim x1).
-  intros. induction on_projs_elim; subst.
-  - cbn. eauto.
+  pose proof (PCUICWeakeningEnv.on_declared_projection X d) as [oni onp].
+  simpl in onp. destruct ind_cshapes as [|? []]; try contradiction.
+  destruct onp as (((? & ?) & ?) & ?).
+  inv o. auto.
 Qed. (* elim_restriction_works_proj *)
 
 Lemma elim_restriction_works_proj `{cf : checker_flags} (Σ : global_env_ext) Γ  p c mind idecl T :
@@ -598,7 +594,7 @@ Proof.
   specialize (X0 Hnth').
   simpl in X0. destruct X0 as [[X0 _] _]. subst m.
   clear e0.
-  set (decli := declared_inductive_inv _ _ _  _ _ _ _ _ _) in *.
+  set (decli := declared_inductive_inv _ _ _ _) in *.
   clear oib. clearbody decli.
   unshelve eapply branch_type_spec in e1; eauto.
   now destruct e1 as [e1 _].
